@@ -84,6 +84,22 @@ Fixpoint Mstacks {T A} {n : A -> M} {m : A -> M}
   | a :: l => Mstack (f a) (Mstacks f l)
   end.
 
+Fixpoint Mstacks' {T A} {n : A -> M} {m : A -> M}
+  (f : forall a, MProp M T (n a) (m a)) (l : list A) {struct l} :
+    MProp M T (Mlist_sum' (n <$> l)) (Mlist_sum' (m <$> l)) :=
+  match l with
+  | [] => Mid mO
+  | a :: l' =>
+    match l' as l return MProp M T (Mlist_sum' (n <$> l)) (Mlist_sum' (m <$> l)) ->
+    MProp M T (Mlist_sum' (n <$> (a :: l))) (Mlist_sum' (m <$> (a :: l))) with 
+    | [] => fun _ => f a
+    | _ => fun st => Mstack (f a) st
+    end (Mstacks' f l')
+  (* | [a] => f a
+  | a :: l => Mstack (f a) (Mstacks' f l) *)
+  end.
+
+
 Definition sizeX (smap : Pmap X) := (λ i, default mO (mdecomp_inv <$> (smap !! i))).
 
 
@@ -179,10 +195,10 @@ Definition mprop_perm_of_empty_sized_graph {T n m} smap
     Heq ← guard (apply_sw (vmap (smap !!.) inputs) 
       ((λ k, default (pos_to_nat_pred k) (list_index k inputs))
         <$> vec_to_list outputs) =@{list _} vmap (smap !!.) outputs);
-    Some (((mprop_of_sw (vmap (sizeX smap) inputs)
+    Some (cast_mprop (reflexivity _) (mprop_perm_of_empty_sized_graph_prf Heq) 
+      ((mprop_of_sw (vmap (sizeX smap) inputs)
       ((λ k, default (pos_to_nat_pred k) (list_index k inputs))
-        <$> vec_to_list outputs))) ;' Massoc' 
-        (mprop_perm_of_empty_sized_graph_prf Heq)).
+        <$> vec_to_list outputs)))).
 
 Lemma sized_graph_to_term_aux_prf {T n smap}
   {es : list (positive * HyperEdge T)} {inputs : vec positive n}
@@ -232,7 +248,7 @@ Fixpoint sized_graph_to_term_aux {T n m} (depth : nat)
       Heq ← guard ((smap !!.) <$> (flat_map (λ tio, tio.2.2) es ++ 
         filter (λ x : positive, x ∉ foldr app [] es.*2.*1.*2) (vec_to_list inputs))
         = (smap !!.) <$> inputs');
-      Some (tl ;' Massoc' (sized_graph_to_term_aux_prf Heq) ;' tr)
+      Some (Mcompose_cast tl tr (sized_graph_to_term_aux_prf Heq))
       (* Mocompose tl tr ≫= ocast_mprop_r _ *)
       (* tl' ← ocast_aprop tl;
       Some (tl' ;' tr)%aprop *)
@@ -249,6 +265,131 @@ Definition sized_graph_to_term {T n m} (scohg : SizedCospanHyperGraph X T n m) :
 
 
 
+Lemma layer_to_aprop_prf' {T n} {smap} {es : list (HyperEdge T)}
+  {inputs : vec positive n} {es_inputs unused_inputs} : 
+  apply_sw inputs ((λ k, default (pos_to_nat_pred k) (list_index k inputs)) <$>
+     es_inputs ++ unused_inputs) =@{list _}
+  flat_map (λ tio, tio.1.2) es ++ unused_inputs ->
+  Mlist_sum' (apply_sw (vmap (sizeX smap) inputs)
+     ((λ k, default (pos_to_nat_pred k) (list_index k inputs)) <$>
+      es_inputs ++ unused_inputs)) ==
+  Mlist_sum' ((λ tio, Mlist_sum' (sizeX smap <$> tio.1.2)) <$> es) +
+  Mlist_sum' (sizeX smap <$> unused_inputs).
+Proof.
+  rewrite 3 Mlist_sum'_correct.
+  intros ->%layer_to_aprop_prf.
+  f_equiv.
+  apply Mlist_sum_perm_mor.
+  apply SetoidList.eqlistA_altdef, Forall2_fmap.
+  apply Forall_Forall2_diag.
+  rewrite Forall_forall.
+  intros; now rewrite Mlist_sum'_correct.
+Qed.
+
+Definition layer_to_mprop' {T n} smap (es : list (HyperEdge T))
+  (inputs : vec positive n) : option (MProp M T
+    (Mlist_sum' (MD:=MD)(vec_to_list (vmap (sizeX smap) inputs)))
+    (Mlist_sum' (MD:=MD) (((λ tio, Mlist_sum' (sizeX smap <$> tio.2)) <$> es))
+    + Mlist_sum' (MD:=MD) (sizeX smap <$> (filter (.∉ foldr app [] es.*1.*2) (vec_to_list inputs))))
+     * list positive) :=
+  (let es_inputs := foldr app [] es.*1.*2 in
+  let es_outputs := foldr app [] es.*2 in
+  let unused_inputs := filter (.∉ es_inputs) (vec_to_list inputs) in
+  let estack := Mstacks' (fun tio =>
+    Mgen tio.1.1 (Mlist_sum' (sizeX smap <$> tio.1.2))
+      (Mlist_sum' (sizeX smap <$> tio.2))) es in
+  let perm := (mprop_of_sw' (vmap (sizeX smap) inputs)
+    ((λ k, default (pos_to_nat_pred k) $ list_index k inputs)
+    <$> (es_inputs ++ unused_inputs))) in
+  Heq ← guard (apply_sw inputs ((λ k, default (pos_to_nat_pred k) $ list_index k inputs)
+    <$> (es_inputs ++ unused_inputs)) =@{list _}
+    flat_map (λ tio, tio.1.2) es ++ unused_inputs);
+  let t := Mcompose_cast perm (Mstack estack (Mid (Mlist_sum' (sizeX smap <$> unused_inputs)))) 
+  (layer_to_aprop_prf' Heq) in
+  Some (t, es_outputs ++ unused_inputs)).
+
+Lemma mprop_perm_of_empty_sized_graph_prf' {n m} {smap}
+  {inputs : vec positive n} {outputs : vec positive m} : 
+  apply_sw (vmap (smap !!.) inputs)
+    ((λ k, default (pos_to_nat_pred k) (list_index k inputs)) <$>
+     (vec_to_list outputs)) =@{list _} vmap (smap !!.) outputs ->
+  Mlist_sum'
+    (apply_sw (vmap (sizeX smap) inputs)
+     ((λ k, default (pos_to_nat_pred k) (list_index k inputs)) <$>
+      (vec_to_list outputs))) == Mlist_sum' (vmap (sizeX smap) outputs).
+Proof.
+  rewrite 2 Mlist_sum'_correct.
+  apply mprop_perm_of_empty_sized_graph_prf.
+Qed.
+
+
+Definition mprop_perm_of_empty_sized_graph' {T n m} smap
+  (inputs : vec positive n) (outputs : vec positive m) :
+    option (MProp M T (Mlist_sum' (vmap (sizeX smap) inputs))
+      (Mlist_sum' (vmap (sizeX smap) outputs))) :=
+    Heq ← guard (apply_sw (vmap (smap !!.) inputs) 
+      ((λ k, default (pos_to_nat_pred k) (list_index k inputs))
+        <$> vec_to_list outputs) =@{list _} vmap (smap !!.) outputs);
+    Some (cast_mprop (reflexivity _) (mprop_perm_of_empty_sized_graph_prf' Heq)
+    ((mprop_of_sw' (vmap (sizeX smap) inputs)
+      ((λ k, default (pos_to_nat_pred k) (list_index k inputs))
+        <$> vec_to_list outputs)))).
+
+Lemma sized_graph_to_term_aux_prf' {T n smap}
+  {es : list (positive * HyperEdge T)} {inputs : vec positive n}
+  {inputs'} :
+  (λ i : positive, smap !! i) <$> flat_map (λ tio : positive * HyperEdge T, tio.2.2) es ++
+  filter (λ x : positive, x ∉ foldr app [] es.*2.*1.*2) (vec_to_list inputs) =
+  (λ i : positive, smap !! i) <$> inputs' ->
+  Mlist_sum' ((λ tio : HyperEdge T, Mlist_sum' (sizeX smap <$> tio.2)) <$> es.*2) +
+  Mlist_sum' (sizeX smap <$> filter (λ x : positive, x ∉ foldr app [] es.*2.*1.*2) (vec_to_list inputs)) ==
+  Mlist_sum' (vmap (sizeX smap) (list_to_vec inputs')).
+Proof.
+  rewrite 3 Mlist_sum'_correct.
+  intros <-%sized_graph_to_term_aux_prf.
+  f_equiv.
+  apply Mlist_sum_perm_mor.
+  apply SetoidList.eqlistA_altdef, Forall2_fmap.
+  apply Forall_Forall2_diag.
+  rewrite Forall_forall.
+  intros; now rewrite Mlist_sum'_correct.
+Qed.
+
+
+Fixpoint sized_graph_to_term_aux' {T n m} (depth : nat)
+  smap
+  (hg : Pmap (HyperEdge T)) (inputs : vec positive n) (outputs : vec positive m) :
+    option (MProp M T (Mlist_sum' (vmap (sizeX smap) inputs))
+      (Mlist_sum' (vmap (sizeX smap) outputs))) :=
+
+  match hg with
+  | PEmpty =>
+    mprop_perm_of_empty_sized_graph' smap inputs outputs
+  | PNodes _ =>
+    match depth with
+    | 0 => None
+    | S depth =>
+      let '(es, (_, hg')) :=
+        get_simultaneously_extractable_edges inputs hg in
+      '(tl, inputs') ← layer_to_mprop' smap es.*2 inputs;
+      tr ← sized_graph_to_term_aux' depth smap hg' (list_to_vec inputs') outputs;
+      Heq ← guard ((smap !!.) <$> (flat_map (λ tio, tio.2.2) es ++ 
+        filter (λ x : positive, x ∉ foldr app [] es.*2.*1.*2) (vec_to_list inputs))
+        = (smap !!.) <$> inputs');
+      Some (Mcompose_cast tl tr (sized_graph_to_term_aux_prf' Heq))
+      (* Mocompose tl tr ≫= ocast_mprop_r _ *)
+      (* tl' ← ocast_aprop tl;
+      Some (tl' ;' tr)%aprop *)
+    end
+  end.
+
+
+
+Definition sized_graph_to_term' {T n m} (scohg : SizedCospanHyperGraph X T n m) :
+  option (MProp M T (Mlist_sum' (vmap (sizeX scohg.(sized_map)) scohg.(inputs)))
+      (Mlist_sum' (vmap (sizeX scohg.(sized_map)) scohg.(outputs)))) :=
+  sized_graph_to_term_aux' (size (hyperedges scohg)) (scohg.(sized_map))
+    (hyperedges scohg) (inputs scohg) (outputs scohg).
 
 
 
@@ -305,27 +446,6 @@ Proof.
   reflexivity.
 Qed.
 
-(* Example test_HG2T_sw120 :
-  correct (sw [1;2;0] :> AProp bool _ _).
-Proof.
-  unfold from_option.
-  case_match eqn:Heq; vm_compute in Heq; [|done].
-  revert Heq.
-  intros [= <-].
-  apply graph_iso_partial_test_correct; vm_compute; done.
-Qed.
-
-
-Example test_HG2T_sw201 :
-  correct (sw [2;0;1] :> AProp bool _ _).
-Proof.
-  unfold from_option.
-  case_match eqn:Heq; vm_compute in Heq; [|done].
-  revert Heq.
-  intros [= <-].
-  apply graph_iso_partial_test_correct; vm_compute; done.
-Qed. *)
-
 
 
 Example test_HG2T_gen11 :
@@ -360,38 +480,70 @@ Proof.
   reflexivity.
 Qed.
 
-(*
-Example bug_case_1 :
-  let G := ([#74%positive; 19%positive] ->
-       mk_hg
-         (list_to_map
-             [(32%positive, (true, [], [68%positive]))])
-         {[19%positive; 74%positive]} <- [#19%positive; 68%positive; 74%positive]) in
-  forall ap,
-  graph_to_term G = Some ap ->
-  G ≡ₛ AProp_graph_semantics ap.
+
+
+Local Notation "'correct_' ap" :=
+  (from_option (λ t, MProp_graph_eq t ap) False
+    (sized_graph_to_term' (MProp_sized_graph_semantics ap) ≫= ocast_mprop _ _ ))
+  (at level 10, only parsing).
+
+Example test_HG2T_Aswap11' :
+  correct_ (Mswap (T:=bool) (bleaf true) (bleaf false)).
 Proof.
-  cbv zeta.
-
-
-  vm_eval (graph_to_term _).
-  intros _ [= <-].
-  apply graph_iso_partial_test_correct.
+  vm_eval (sized_graph_to_term' _).
+  cbn.
+  vm_eval (ocast_mprop _ _ _).
+  cbn.
+  apply sized_graph_iso_partial_test_correct.
   vm_compute.
-  done.
+  reflexivity.
+Qed.
 
-  (* unfold graph_to_term.
-  vm_compute (sizeX _).
-  unfold graph_to_term_aux.
-  vm_eval (hyperedges _).
-  vm_eval (get_simultaneously_extractable_edges _ _).
-  vm_eval (inputs _).
-  unfold layer_to_aprop.
-  vm_eval (fmap (M:=list) _ _).
-  vm_eval (fmap (M:=list) _ _).
-  vm_eval (layer_to_aprop _ _).
-  cbn. *)
-Qed. *)
+Example test_HG2T_sw120_alt' :
+  correct_ (Mswap (bleaf true) (bleaf false) *
+    Mid (T:=bool) (bnode (bleaf true) (bleaf false)) ;''
+    Mid (T:=bool) (bleaf false) * Mswap (bnode (bleaf true) (bleaf true)) (bleaf false))%mprop.
+Proof.
+  vm_eval (mbind _ _);
+  cbn;
+  apply sized_graph_iso_partial_test_correct;
+  vm_compute;
+  reflexivity.
+Qed.
+
+
+
+Example test_HG2T_gen11' :
+  correct_ (Mgen true (bleaf true) (bleaf false)).
+Proof.
+  vm_eval (mbind _ _);
+  cbn;
+  apply sized_graph_iso_partial_test_correct;
+  vm_compute;
+  reflexivity.
+Qed.
+
+Example test_HG2T_gen11_11' :
+  correct_ (Mgen true (bleaf false) (bleaf true) ;' Mgen false (bleaf true) (bleaf true)).
+Proof.
+  vm_eval (mbind _ _);
+  cbn;
+  apply sized_graph_iso_partial_test_correct;
+  vm_compute;
+  reflexivity.
+Qed.
+
+
+Example test_HG2T_gen12_11' :
+  correct_ (Mgen true (bempty) (bnode (bleaf true) (bleaf false)) ;' Mgen false (bleaf true) (bleaf false) * Mid (bleaf false)).
+Proof.
+
+  vm_eval (mbind _ _);
+  cbn;
+  apply sized_graph_iso_partial_test_correct;
+  vm_compute;
+  reflexivity.
+Qed.
 
 
 
